more structure in monad examples

examples/Basics/DY.Basics.Monads.fst
@@ -4,7 +4,7 @@ open Comparse
 open DY.Core
 open DY.Lib
 
-#set-options "--fuel 0 --ifuel 1 --z3rlimit 25  --z3cliopt 'smt.qi.eager_threshold=100'"
+#set-options "--fuel 3 --ifuel 1 --z3rlimit 25  --z3cliopt 'smt.qi.eager_threshold=100'"
 
 #push-options "--fuel 1"
 val add_entry_: trace_entry -> traceful (option unit)
@@ -15,6 +15,9 @@ let add_entry_ e tr =
 #pop-options
 
 let en = Corrupt 1
+
+
+(*** Composition in the traceful + option monad ***)
 
 let f (x:int) : traceful (option string) =
   if x < 2 
@@ -44,30 +47,6 @@ let f3''' :traceful (option string) =
   f 0;*?
   f 1
 
-let f3_tr :traceful (option string) = 
-  f 1;*
-  f 2;*
-  f 0
-
-let f3_ :traceful (option string) = 
-  f 1;*?
-  f 2;*
-  f 0
-
-let f3_' :traceful (option string) = 
-  f 1;*
-  f 3;*
-  f 1;*
-  f 2;*?
-  f 0
-
-let f3_'' :traceful (option string) = 
-  f 1;*
-  f 3;*?
-  f 1;*
-  f 2;*?
-  f 0
-
 
 let rec trace_from_rev_list (ens: list trace_entry) : trace =
   match ens with
@@ -78,7 +57,6 @@ open FStar.List.Tot.Base
 
 let trace_from_list ens = trace_from_rev_list (rev ens)
 
-#push-options "--fuel 3"
 let _ = 
   let ev1 = Corrupt 1 in
   let ev2 = Corrupt 2 in
@@ -109,9 +87,7 @@ let _ =
   assert(None? opt_s_ges);
   assert(t_ges == trace_from_list [en]);
 
-  let (opt_s_ges, t_ges) = f3_tr t in
-  assert(Some? opt_s_ges);
-  assert(t_ges == trace_from_list [en;en]);
+ 
 
   let (opt_s_ges, t_ges) = f3' t in
   assert(None? opt_s_ges);
@@ -125,6 +101,120 @@ let _ =
   assert(Some? opt_s_ges);
   assert(t_ges == trace_from_list [en; en]);
 
+
+  ()
+
+(*** Comparing traceful+option with plain traceful actions ***)
+
+
+let f3_tr :traceful (option string) = 
+  f 1;*
+  f 2;*
+  f 0
+
+
+let _ = 
+  let t = trace_from_list [] in
+
+  let (opt_s_ges, t_ges) = f3_tr t in
+  assert(Some? opt_s_ges);
+  assert(t_ges == trace_from_list [en;en]);
+  ()
+
+
+(*** Combining traceful+option with option actions ***)
+
+val f_opt: nat -> option nat
+let f_opt n =
+  if n < 2 
+  then None
+  else Some (n-1)
+
+val f_combine_tropt_and_opt: nat -> traceful (option string)
+let f_combine_tropt_and_opt n =
+  return (f_opt n);*?
+  f n
+
+(*** Combining traceful+option with plain non-optional traceful actions ***)
+
+let entr x = Corrupt x
+
+val f_tr_nonopt: nat -> traceful nat
+let f_tr_nonopt x =
+  add_entry (entr x);*
+  return (x + 1 <: nat)
+
+val f_combine_tropt_and_trnonopt: nat -> traceful (option string)
+let f_combine_tropt_and_trnonopt x =
+  f_tr_nonopt x;*
+  f x
+
+val f_combine_tropt_and_trnonopt_with_let: nat -> traceful (option string)
+let f_combine_tropt_and_trnonopt_with_let x =
+  let* nx = f_tr_nonopt x in
+  f nx
+
+
+val f_combine_tropt_and_trnonopt_more: nat -> traceful (option nat)
+let f_combine_tropt_and_trnonopt_more x =
+  let* nx = f_tr_nonopt x in
+  f nx;*?
+  let* nnx = f_tr_nonopt nx in
+  return (Some nnx)
+
+#push-options "--fuel 4"
+let _ =
+  let t = trace_from_list [] in
+  let x = 0 in
+
+  let (nx, tr) = f_tr_nonopt x t in
+  assert(nx = 1);
+  assert(tr == trace_from_list [entr x] );
+
+
+  let (opt_str, tr_opt) = f_combine_tropt_and_trnonopt x t in
+  assert(Some? opt_str);
+  assert(tr_opt == trace_from_list [entr x; en]);
+
+  let (opt_str, tr_opt) = f_combine_tropt_and_trnonopt_with_let 1 t in
+  assert(None? opt_str);
+  assert(tr_opt == trace_from_list [entr 1]);
+  
+  let (opt_n, tr_opt) = f_combine_tropt_and_trnonopt_more 0 t in
+  assert(opt_n = Some 2);
+  assert(tr_opt == trace_from_list [entr 0; en; entr 1]);
+  
+  
+  let (opt_str, tr_opt) = f_combine_tropt_and_trnonopt_more 1 t in
+  assert(None? opt_str);
+  assert(tr_opt == trace_from_list [entr 1]);
+  ()
+#pop-options
+
+(*** Combining traceful+option with traceful actions ***)
+
+let f3_ :traceful (option string) = 
+  f 1;*?
+  f 2;*
+  f 0
+
+let f3_' :traceful (option string) = 
+  f 1;*
+  f 3;*
+  f 1;*
+  f 2;*?
+  f 0
+
+let f3_'' :traceful (option string) = 
+  f 1;*
+  f 3;*?
+  f 1;*
+  f 2;*?
+  f 0
+
+let _ =
+  let t = trace_from_list [] in
+  
   let (opt_s_ges, t_ges) = f3_ t in
   assert(Some? opt_s_ges);
   assert(t_ges == trace_from_list [en; en]);
@@ -136,6 +226,4 @@ let _ =
   let (opt_s_ges, t_ges) = f3_'' t in
   assert(None? opt_s_ges);
   assert(t_ges == trace_from_list [en]);
-
   ()
-#pop-options
